Equivalence proof for networks with state

Networks.thy
@@ -13,45 +13,47 @@ text \<open>Input, output and internal transitions\<close>
 
 datatype 'a act = In 'a | Out 'a | Sil 'a
 
+datatype 'b label = Del | Act 'b | Syn 'b 'b
+
 type_synonym
-  ('a, 'c, 't, 's) nta = "('a act, 'c, 't, 's) ta list"
+  ('a, 'b, 'c, 't, 's) nta = "('a act * 'b, 'c, 't, 's) ta list"
 
 inductive step_n ::
-  "('a, 'c, 't, 's) nta \<Rightarrow> 's list \<Rightarrow> ('c, ('t::time)) cval
+  "('a, 'b, 'c, 't, 's) nta \<Rightarrow> 's list \<Rightarrow> ('c, ('t::time)) cval \<Rightarrow> 'b label
   \<Rightarrow> 's list \<Rightarrow> ('c, 't) cval \<Rightarrow> bool"
-("_ \<turnstile>\<^sub>N \<langle>_, _\<rangle> \<rightarrow> \<langle>_,_\<rangle>" [61,61,61] 61)
+("_ \<turnstile>\<^sub>N \<langle>_, _\<rangle> \<rightarrow>\<^bsub>_\<^esub> \<langle>_,_\<rangle>" [61,61,61,61,61,61] 61)
 where
   step_n_t:
     "\<lbrakk>\<forall> p \<in> {..<length N}. N!p \<turnstile> \<langle>L!p, u\<rangle> \<rightarrow>\<^bsup>d\<^esup> \<langle>L!p, u \<oplus> d\<rangle>; d \<ge> 0\<rbrakk>
-    \<Longrightarrow> N \<turnstile>\<^sub>N \<langle>L, u\<rangle> \<rightarrow> \<langle>L, u \<oplus> d\<rangle>" |
+    \<Longrightarrow> N \<turnstile>\<^sub>N \<langle>L, u\<rangle> \<rightarrow>\<^bsub>Del\<^esub> \<langle>L, u \<oplus> d\<rangle>" |
   step_n_i:
     "\<lbrakk>
-      N!p \<turnstile> l \<longrightarrow>\<^bsup>g,Sil a,r\<^esup> l'; u \<turnstile> g; \<forall> p \<in> {..<length N}. u' \<turnstile> inv_of (N!p) (L'!p);
+      N!p \<turnstile> l \<longrightarrow>\<^bsup>g,(Sil a, b),r\<^esup> l'; u \<turnstile> g; \<forall> p \<in> {..<length N}. u' \<turnstile> inv_of (N!p) (L'!p);
       L!p = l; p < length L; L' = L[p := l']; u' = [r\<rightarrow>0]u
      \<rbrakk>
-    \<Longrightarrow> N \<turnstile>\<^sub>N \<langle>L, u\<rangle> \<rightarrow> \<langle>L', u'\<rangle>" |
+    \<Longrightarrow> N \<turnstile>\<^sub>N \<langle>L, u\<rangle> \<rightarrow>\<^bsub>Act b\<^esub> \<langle>L', u'\<rangle>" |
   step_n_s:
-    "\<lbrakk>N!p \<turnstile> l1 \<longrightarrow>\<^bsup>g1,In a,r1\<^esup> l1'; N!q \<turnstile> l2 \<longrightarrow>\<^bsup>g2,Out a,r2\<^esup> l2'; u \<turnstile> g1; u \<turnstile> g2;
+    "\<lbrakk>N!p \<turnstile> l1 \<longrightarrow>\<^bsup>g1,(In a, b1),r1\<^esup> l1'; N!q \<turnstile> l2 \<longrightarrow>\<^bsup>g2,(Out a, b2),r2\<^esup> l2'; u \<turnstile> g1; u \<turnstile> g2;
       \<forall> p \<in> {..<length N}. u' \<turnstile> inv_of (N!p) (L'!p);
       L!p = l1; L!q = l2; p < length L; q < length L; p \<noteq> q;
       L' = L[p := l1', q := l2']; u' = [(r1 @ r2)\<rightarrow>0]u
-     \<rbrakk> \<Longrightarrow> N \<turnstile>\<^sub>N \<langle>L, u\<rangle> \<rightarrow> \<langle>L', u'\<rangle>"
+     \<rbrakk> \<Longrightarrow> N \<turnstile>\<^sub>N \<langle>L, u\<rangle> \<rightarrow>\<^bsub>Syn b1 b2\<^esub> \<langle>L', u'\<rangle>"
 
-inductive_cases[elim!]: "N \<turnstile>\<^sub>N \<langle>L, u\<rangle> \<rightarrow> \<langle>L', u'\<rangle>"
+inductive_cases[elim!]: "N \<turnstile>\<^sub>N \<langle>L, u\<rangle> \<rightarrow>\<^bsub>a\<^esub> \<langle>L', u'\<rangle>"
 
 inductive steps_n ::
-  "('a, 'c, 't, 's) nta \<Rightarrow> 's list \<Rightarrow> ('c, ('t::time)) cval
+  "('a, 'b, 'c, 't, 's) nta \<Rightarrow> 's list \<Rightarrow> ('c, ('t::time)) cval
   \<Rightarrow> 's list \<Rightarrow> ('c, 't) cval \<Rightarrow> bool"
 ("_ \<turnstile>\<^sub>N \<langle>_, _\<rangle> \<rightarrow>* \<langle>_,_\<rangle>" [61,61,61] 61)
 where
   refl: "N \<turnstile>\<^sub>N \<langle>l, Z\<rangle> \<rightarrow>* \<langle>l, Z\<rangle>" |
-  step: "N \<turnstile>\<^sub>N \<langle>l, Z\<rangle> \<rightarrow>* \<langle>l', Z'\<rangle> \<Longrightarrow> N \<turnstile>\<^sub>N \<langle>l', Z'\<rangle> \<rightarrow> \<langle>l'', Z''\<rangle>
+  step: "N \<turnstile>\<^sub>N \<langle>l, Z\<rangle> \<rightarrow>* \<langle>l', Z'\<rangle> \<Longrightarrow> N \<turnstile>\<^sub>N \<langle>l', Z'\<rangle> \<rightarrow>\<^bsub>_\<^esub> \<langle>l'', Z''\<rangle>
         \<Longrightarrow> N \<turnstile>\<^sub>N \<langle>l, Z\<rangle> \<rightarrow>* \<langle>l'', Z''\<rangle>"
 
 declare steps_n.intros[intro]
 
 lemma stepI2:
-  "N \<turnstile>\<^sub>N \<langle>l, Z\<rangle> \<rightarrow>* \<langle>l'', Z''\<rangle>" if "N \<turnstile>\<^sub>N \<langle>l', Z'\<rangle> \<rightarrow>* \<langle>l'', Z''\<rangle>" "N \<turnstile>\<^sub>N \<langle>l, Z\<rangle> \<rightarrow> \<langle>l', Z'\<rangle>"
+  "N \<turnstile>\<^sub>N \<langle>l, Z\<rangle> \<rightarrow>* \<langle>l'', Z''\<rangle>" if "N \<turnstile>\<^sub>N \<langle>l', Z'\<rangle> \<rightarrow>* \<langle>l'', Z''\<rangle>" "N \<turnstile>\<^sub>N \<langle>l, Z\<rangle> \<rightarrow>\<^bsub>b\<^esub> \<langle>l', Z'\<rangle>"
   using that
   apply induction
    apply rule
@@ -63,7 +65,7 @@ lemma stepI2:
 lemma step_n_t_I:
   "\<lbrakk>\<forall> p \<in> {..<length N}. u \<turnstile> inv_of (N!p) (L!p); \<forall> p \<in> {..<length N}. u \<oplus> d \<turnstile> inv_of (N!p) (L!p);
     d \<ge> 0
-   \<rbrakk> \<Longrightarrow> N \<turnstile>\<^sub>N \<langle>L, u\<rangle> \<rightarrow> \<langle>L, u \<oplus> d\<rangle>"
+   \<rbrakk> \<Longrightarrow> N \<turnstile>\<^sub>N \<langle>L, u\<rangle> \<rightarrow>\<^bsub>Del\<^esub> \<langle>L, u \<oplus> d\<rangle>"
 by (auto intro: step_n_t)
 
 subsection \<open>Product Automaton\<close>
@@ -93,7 +95,7 @@ lemma list_update_nth_split:
     using assms by (cases "i = j") auto
 
 locale Product_TA_Defs =
-  fixes N :: "('a, 'c, 't, 's) nta"
+  fixes N :: "('a, 'b, 'c, 't, 's) nta"
 begin
 
   abbreviation "T \<equiv> map trans_of N"
@@ -103,22 +105,47 @@ begin
 
   definition
     "product_trans_i =
-      {(L,g,a,r,L[p:=l']) | L p g a r l'. L \<in> states \<and> (L!p, g, Sil a, r, l') \<in> T!p \<and> p < length L}"
+      {(L,g,(a,Act b),r,L[p:=l']) | L p g a b r l'.
+      L \<in> states \<and> (L!p, g, (Sil a, b), r, l') \<in> T!p \<and> p < length L}"
 
   definition
     "product_trans_s =
-      {(L,g1 @ g2,a,r1 @ r2,L[p:=l1',q:=l2']) | L p q g1 g2 a r1 r2 l1' l2'.
-        L \<in> states \<and> (L!p, g1, In a, r1, l1') \<in> T!p \<and> (L!q, g2, Out a, r2, l2') \<in> T!q
+      {(L,g1 @ g2,(a,Syn b1 b2),r1 @ r2,L[p:=l1',q:=l2']) | L p q g1 g2 a b1 b2 r1 r2 l1' l2'.
+        L \<in> states \<and> (L!p, g1, (In a, b1), r1, l1') \<in> T!p \<and> (L!q, g2, (Out a, b2), r2, l2') \<in> T!q
         \<and> p < length L \<and> q < length L \<and> p \<noteq> q
       }"
 
   definition
     "product_trans \<equiv> product_trans_i \<union> product_trans_s"
+  
+lemma *:
+  "length T = length N"
+  by simp
+  
+lemma product_state_set_subs:
+  assumes "q < length N" "l \<in> state_set product_trans"
+  shows "l ! q \<in> state_set (T ! q)"
+  using assms
+  unfolding product_trans_def product_trans_i_def product_trans_s_def states_def
+  apply safe
+     apply (auto; fail)
+    apply (auto; fail)
+  apply simp
+   apply (subst list_update_nth_split; force) (* XXX Slow *)
+  apply simp
+  apply (subst list_update_nth_split)
+   apply simp
+  apply safe
+   apply (subst (asm) (2) list_update_nth_split; force)
+  apply (subst list_update_nth_split)
+   apply simp
+  by (subst (asm) (2) list_update_nth_split; force)  (* XXX Slow *)
 
   definition
-    "product_invariant L \<equiv> concat (map (\<lambda> p. if p < length I then (I!p) (L!p) else []) [0..<length L])"
+    "product_invariant L \<equiv>
+    concat (map (\<lambda> p. if p < length I then (I!p) (L!p) else []) [0..<length L])"
 
-  definition product_ta :: "('a, 'c, 't, 's list) ta" where
+  definition product_ta :: "('a \<times> 'b label, 'c, 't, 's list) ta" where
     "product_ta \<equiv> (product_trans, product_invariant)"
 
   lemma collect_clki_product_invariant:
@@ -183,28 +210,28 @@ begin
 
   lemma product_trans_s_alt_def:
     "product_trans_s =
-      {(L, g, a, r, L') | L g a r L'. \<exists> p q g1 g2 r1 r2 l1' l2'.
+      {(L, g, (a, Syn b1 b2), r, L') | L g a b1 b2 r L'. \<exists> p q g1 g2 r1 r2 l1' l2'.
       L \<in> states \<and> p < length L \<and> q < length L \<and> p \<noteq> q \<and>
       g = g1 @ g2 \<and> r = r1 @ r2 \<and> L' = L[p:=l1', q:=l2']
-        \<and> (L!p, g1, In a, r1, l1') \<in> T!p \<and> (L!q, g2, Out a, r2, l2') \<in> T!q
+        \<and> (L!p, g1, (In a, b1), r1, l1') \<in> T!p \<and> (L!q, g2, (Out a, b2), r2, l2') \<in> T!q
       }"
     unfolding product_trans_s_def by (safe; metis)
-  
+
   context
     assumes states_not_empty: "states \<noteq> {}"
     assumes trans_complete:
-      "\<forall> p < length T. \<forall> t1 \<in> T ! p. case t1 of (l1, g1, In a, r1, l1')
-      \<Rightarrow> \<exists> q < length T. p \<noteq> q \<and> (\<exists> l2 g2 r2 l2'. (l2, g2, Out a, r2, l2') \<in> T ! q) |
-      (l1, g1, Out a, r1, l1')
-      \<Rightarrow> \<exists> q < length T. p \<noteq> q \<and> (\<exists> l2 g2 r2 l2'. (l2, g2, In a, r2, l2') \<in> T ! q) | _ \<Rightarrow> True"
+      "\<forall> p < length T. \<forall> t1 \<in> T ! p. case t1 of (l1, g1, (In a, b1), r1, l1')
+      \<Rightarrow> \<exists> q < length T. p \<noteq> q \<and> (\<exists> l2 g2 b2 r2 l2'. (l2, g2, (Out a, b2), r2, l2') \<in> T ! q) |
+      (l1, g1, (Out a, b1), r1, l1')
+      \<Rightarrow> \<exists> q < length T. p \<noteq> q \<and> (\<exists> l2 g2 b2 r2 l2'. (l2, g2, (In a, b2), r2, l2') \<in> T ! q) | _ \<Rightarrow> True"
   begin
 
   lemma collect_clkt_product_trans_sups:
     "collect_clkt product_trans \<supseteq> \<Union> (collect_clkt ` set T)"
   proof
     fix x assume "x \<in> \<Union> (collect_clkt ` set T)"
-    then obtain trans l1 g1 a' r1 l1' where x:
-      "trans \<in> set T" "(l1, g1, a', r1, l1') \<in> trans" "x \<in> collect_clock_pairs g1"
+    then obtain trans l1 g1 a' b1 r1 l1' where x:
+      "trans \<in> set T" "(l1, g1, (a', b1), r1, l1') \<in> trans" "x \<in> collect_clock_pairs g1"
       unfolding collect_clkt_def by force
     then obtain p where p:
         "p < length T" "T ! p = trans"
@@ -214,15 +241,15 @@ begin
     show "x \<in> collect_clkt product_trans"
     proof (cases a')
       case a': (In a)
-      with x p trans_complete obtain q l2 g2 r2 l2' where trans2:
-        "q < length T" "(l2, g2, Out a, r2, l2') \<in> T ! q" "p \<noteq> q"
+      with x p trans_complete obtain q l2 g2 b2 r2 l2' where trans2:
+        "q < length T" "(l2, g2, (Out a, b2), r2, l2') \<in> T ! q" "p \<noteq> q"
         by atomize_elim fastforce
       have "L[p := l1, q := l2] \<in> states" (is "?L \<in> _")
         using L p(1) x(1,2) trans2 unfolding p(2)[symmetric] by (auto intro!: statesI_aux)
       moreover have "?L ! p = l1" "?L ! q = l2"
         using \<open>p \<noteq> q\<close> \<open>p < length T\<close> \<open>q < length T\<close> \<open>L \<in> states\<close> by (auto dest: states_length)
       moreover note t = calculation
-      have "(?L, g1 @ g2, a, r1 @ r2, ?L[p := l1', q := l2']) \<in> product_trans_s"
+      have "(?L, g1 @ g2, (a, Syn b1 b2), r1 @ r2, ?L[p := l1', q := l2']) \<in> product_trans_s"
         unfolding product_trans_s_alt_def
         apply clarsimp
         using t p(1) x(1,2) trans2 unfolding p(2)[symmetric] a' \<open>length T = length L\<close>
@@ -232,15 +259,15 @@ begin
       ultimately show ?thesis unfolding collect_clkt_def product_trans_def by force
     next
       case a': (Out a)
-      with x p trans_complete obtain q l2 g2 r2 l2' where trans2:
-        "q < length T" "(l2, g2, In a, r2, l2') \<in> T ! q" "p \<noteq> q"
+      with x p trans_complete obtain q l2 g2 b2 r2 l2' where trans2:
+        "q < length T" "(l2, g2, (In a, b2), r2, l2') \<in> T ! q" "p \<noteq> q"
         by atomize_elim fastforce
       have "L[q := l2, p := l1] \<in> states" (is "?L \<in> _")
         using L p(1) x(1,2) trans2 unfolding p(2)[symmetric] by (auto intro!: statesI_aux)
       moreover have "?L ! p = l1" "?L ! q = l2"
         using \<open>p \<noteq> q\<close> \<open>p < length T\<close> \<open>q < length T\<close> \<open>L \<in> states\<close> by (auto dest: states_length)
       moreover note t = calculation
-      have "(?L, g2 @ g1, a, r2 @ r1, ?L[q := l2', p := l1']) \<in> product_trans_s"
+      have "(?L, g2 @ g1, (a, Syn b2 b1), r2 @ r1, ?L[q := l2', p := l1']) \<in> product_trans_s"
         unfolding product_trans_s_alt_def
         apply clarsimp
         using t p(1) x(1,2) trans2 unfolding p(2)[symmetric] a' \<open>length T = length L\<close>
@@ -254,7 +281,7 @@ begin
         using L p(1) x(1,2) unfolding p(2)[symmetric] by (auto intro!: statesI_aux)
       moreover have "?L ! p = l1"
         using \<open>p < length T\<close> \<open>L \<in> states\<close> by (auto dest: states_length)
-      ultimately have "(?L, g1, a, r1, ?L[p := l1']) \<in> product_trans_i"
+      ultimately have "(?L, g1, (a, Act b1), r1, ?L[p := l1']) \<in> product_trans_i"
         using x p unfolding product_trans_i_def a' by (force simp: states_length[OF \<open>L \<in> states\<close>])
       with x(3) show ?thesis unfolding collect_clkt_def product_trans_def by force
     qed
@@ -264,8 +291,8 @@ begin
     "collect_clkvt product_trans \<supseteq> \<Union> (collect_clkvt ` set T)"
   proof
     fix x assume "x \<in> \<Union> (collect_clkvt ` set T)"
-    then obtain trans l1 g1 a' r1 l1' where x:
-      "trans \<in> set T" "(l1, g1, a', r1, l1') \<in> trans" "x \<in> set r1"
+    then obtain trans l1 g1 a' b1 r1 l1' where x:
+      "trans \<in> set T" "(l1, g1, (a', b1), r1, l1') \<in> trans" "x \<in> set r1"
       unfolding collect_clkvt_def by force
     then obtain p where p:
         "p < length T" "T ! p = trans"
@@ -274,29 +301,38 @@ begin
     show "x \<in> collect_clkvt product_trans"
     proof (cases a')
       case a': (In a)
-      with x p trans_complete obtain q l2 g2 r2 l2' where trans2:
-        "q < length T" "(l2, g2, Out a, r2, l2') \<in> T ! q" "p \<noteq> q"
+      with x p trans_complete obtain q l2 g2 b2 r2 l2' where trans2:
+        "q < length T" "(l2, g2, (Out a, b2), r2, l2') \<in> T ! q" "p \<noteq> q"
         by atomize_elim fastforce
       moreover have "L[p := l1, q := l2] \<in> states" (is "?L \<in> _")
         using L p(1) x(1,2) trans2 unfolding p(2)[symmetric] by (auto intro!: statesI_aux)
       moreover have "?L ! p = l1" "?L ! q = l2"
         using \<open>p \<noteq> q\<close> \<open>p < length T\<close> \<open>q < length T\<close> \<open>L \<in> states\<close> by (auto dest: states_length)
-      ultimately have "(?L, g1 @ g2, a, r1 @ r2, ?L[p := l1', q := l2']) \<in> product_trans_s"
+      ultimately have
+        "(?L, g1 @ g2, (a, Syn b1 b2), r1 @ r2, ?L[p := l1', q := l2']) \<in> product_trans_s"
         using p(1) x trans2 unfolding p(2)[symmetric] a' product_trans_s_def
         by (fastforce simp: states_length[OF \<open>L \<in> states\<close>])
       with x(3) show ?thesis unfolding collect_clkvt_def product_trans_def by force
     next
       case a': (Out a)
-      with x p trans_complete obtain q l2 g2 r2 l2' where trans2:
-        "q < length T" "(l2, g2, In a, r2, l2') \<in> T ! q" "p \<noteq> q"
+      with x p trans_complete obtain q l2 g2 b2 r2 l2' where trans2:
+        "q < length T" "(l2, g2, (In a, b2), r2, l2') \<in> T ! q" "p \<noteq> q"
         by atomize_elim fastforce
       moreover have "L[q := l2, p := l1] \<in> states" (is "?L \<in> _")
         using L p(1) x(1,2) trans2 unfolding p(2)[symmetric] by (auto intro!: statesI_aux)
       moreover have "?L ! p = l1" "?L ! q = l2"
         using \<open>p \<noteq> q\<close> \<open>p < length T\<close> \<open>q < length T\<close> \<open>L \<in> states\<close> by (auto dest: states_length)
-      ultimately have "(?L, g2 @ g1, a, r2 @ r1, ?L[q := l2', p := l1']) \<in> product_trans_s"
+      ultimately have "(?L, g2 @ g1, (a, Syn b2 b1), r2 @ r1, ?L[q := l2', p := l1']) \<in> product_trans_s"
         using p(1) x trans2 unfolding p(2)[symmetric] a' product_trans_s_def
+        apply (simp add: states_length[OF \<open>L \<in> states\<close>] del: ex_simps)
+        apply (tactic \<open>rearrange_ex_tac @{context} 1\<close>)
+        apply simp
+        apply (rule exI, rule conjI, assumption)
+        apply (simp only: ex_simps[symmetric])
+        apply (tactic \<open>rearrange_ex_tac @{context} 1\<close>)
+        apply simp
         by (fastforce simp: states_length[OF \<open>L \<in> states\<close>])
+          (* fastforce can solve this on its own but not very quickly *)
       with x(3) show ?thesis unfolding collect_clkvt_def product_trans_def by force
     next
       case a': (Sil a)
@@ -304,7 +340,7 @@ begin
         using L p(1) x(1,2) unfolding p(2)[symmetric] by (auto intro!: statesI_aux)
       moreover have "?L ! p = l1"
         using \<open>p < length T\<close> \<open>L \<in> states\<close> by (auto dest: states_length)
-      ultimately have "(?L, g1, a, r1, ?L[p := l1']) \<in> product_trans_i"
+      ultimately have "(?L, g1, (a, Act b1), r1, ?L[p := l1']) \<in> product_trans_i"
         using x p unfolding product_trans_i_def a' by (force simp: states_length[OF \<open>L \<in> states\<close>])
       with x(3) show ?thesis unfolding collect_clkvt_def product_trans_def by force
     qed
@@ -346,10 +382,10 @@ begin
     "finite product_trans_i"
   proof -
     let ?N = "\<Union> (trans_of ` set N)"
-    let ?S = "{(L, p, g, a, r, l')|L p g a r l'.
-      L \<in> states \<and> (L ! p, g, Sil a, r, l') \<in> map trans_of N ! p \<and> p < length L}"
-    let ?R = "{(L, p, g, a, r, l')|L p g a r l'.
-      L \<in> states \<and> p < length L \<and> (g, Sil a, r, l') \<in> snd ` ?N}"
+    let ?S = "{(L, p, g, (a, Act b), r, l')|L p g a b r l'.
+      L \<in> states \<and> (L ! p, g, (Sil a, b), r, l') \<in> map trans_of N ! p \<and> p < length L}"
+    let ?R = "{(L, p, g, (a, Act b), r, l')|L p g a b r l'.
+      L \<in> states \<and> p < length L \<and> (g, (Sil a, b), r, l') \<in> snd ` ?N}"
     have "?S \<subseteq> ?R" by (fastforce simp: states_length dest: nth_mem)
     moreover have "finite ?R" using finite_states [[simproc add: finite_Collect]]
       apply simp
@@ -373,9 +409,7 @@ begin
       unfolding product_trans_i_def apply (rule; rule)
        apply simp
        apply safe[]
-      subgoal for a aa ab ac b L p g ad r l'
-        apply (rule image_eqI[where x = "(L, p, g, ad, r, l')"])
-        by auto
+       apply (fastforce simp: image_Collect)
       by force
     ultimately show ?thesis by auto
   qed
@@ -392,19 +426,16 @@ lemma
   using assms
   using [[simproc add: finite_Collect]] apply simp
   oops
-  
+
   thm Finite_Set.finite_Collect_bounded_ex
-lemma rewr:
-    "\<exists>x. P1 \<and> Q1 x \<equiv> P1 \<and> (\<exists>x. Q1 x)"
-  by simp
-  
+
 lemma
   assumes A: "finite A"
   shows "finite {t. \<exists> a c. a \<in> A \<and> P c \<and> t = (a,c)}"
   using [[simp_trace]] apply simp
   oops
-  
-  
+
+
   (*
   lemma finite_product_trans_s:
     "finite product_trans_s"
@@ -431,7 +462,7 @@ lemma
       oops
       supply [[simproc del: ex_reorder]]
       apply simp
-      
+
     define F1 where "F1 \<equiv> {(g1, a, r1, l1') | g1 a r1 l1'. (g1, In a, r1, l1') \<in> snd ` ?N}"
     have fin1: "finite F1" unfolding F1_def using finite_trans
       using [[simproc add: finite_Collect]] by (auto simp: inj_on_def intro: finite_vimageI)
@@ -468,50 +499,61 @@ lemma
   qed
 *)
 
+  lemma finite_Collect_bounded_ex_5' [simp]:
+  assumes "finite {(a,b,c,d,e) . P a b c d e}"
+  shows
+    "finite {x. \<exists>a b c d e. P a b c d e \<and> Q x a b c d e}
+    \<longleftrightarrow> (\<forall> a b c d e. P a b c d e \<longrightarrow> finite {x. Q x a b c d e})"
+  using assms finite_Collect_bounded_ex[OF assms, where Q = "\<lambda> x. \<lambda> (a, b, c, d, e). Q x a b c d e"]
+  by clarsimp (* force, simp *)
+  
   lemma finite_product_trans_s:
     "finite product_trans_s"
   proof -
     let ?N = "\<Union> (trans_of ` set N)"
     (* XXX Possible intro weakening for finiteness method *)
-    have "(g1, In a, r1, l1') \<in> snd ` ?N" if
-      "(L ! p, g1, In a, r1, l1') \<in> map trans_of N ! p" "p < length L" "L \<in> states"
-      for L p g1 a r1 l1'
+    have "(g1, (In a, b), r1, l1') \<in> snd ` ?N" if
+      "(L ! p, g1, (In a, b), r1, l1') \<in> map trans_of N ! p" "p < length L" "L \<in> states"
+      for L p g1 a b r1 l1'
       using that by (auto simp: states_length dest: nth_mem)
-    let ?S = "{(L, p, q, g1, g2, a, r1, r2, l1', l2')|L p q g1 g2 a r1 r2 l1' l2'.
-      L \<in> states \<and> (L ! p, g1, In a, r1, l1') \<in> map trans_of N ! p \<and>
-        (L ! q, g2, Out a, r2, l2') \<in> map trans_of N ! q \<and> p < length L \<and> q < length L}"
-    define F1 where "F1 \<equiv> {(g1, a, r1, l1') | g1 a r1 l1'. (g1, In a, r1, l1') \<in> snd ` ?N}"
+    let ?S = "{(L, p, q, g1, g2, (a, Syn b1 b2), r1, r2, l1', l2')|L p q g1 g2 a b1 b2 r1 r2 l1' l2'.
+      L \<in> states \<and> (L ! p, g1, (In a, b1), r1, l1') \<in> map trans_of N ! p \<and>
+        (L ! q, g2, (Out a, b2), r2, l2') \<in> map trans_of N ! q \<and> p < length L \<and> q < length L}"
+    define F1 where "F1 \<equiv> {(g1, a, b, r1, l1') | g1 a b r1 l1'. (g1, (In a, b), r1, l1') \<in> snd ` ?N}"
     have fin1: "finite F1" unfolding F1_def using finite_trans
-      using [[simproc add: finite_Collect]] by (auto simp: inj_on_def intro: finite_vimageI)
-    define F2 where "F2 \<equiv> {(g1, a, r1, l1') | g1 a r1 l1'. (g1, Out a, r1, l1') \<in> snd ` ?N}"
+      using [[simproc add: finite_Collect]] by (force simp: inj_on_def intro: finite_vimageI)
+    define F2 where "F2 \<equiv> {(g1, a, b, r1, l1') | g1 a b r1 l1'. (g1, (Out a, b), r1, l1') \<in> snd ` ?N}"
     have fin2: "finite F2" unfolding F2_def using finite_trans
-      using [[simproc add: finite_Collect]] by (auto simp: inj_on_def intro: finite_vimageI)
-    define R where "R \<equiv> {(L, p, q, g1, g2, a, r1, r2, l1', l2')|L p q g1 g2 a r1 r2 l1' l2'.
-      L \<in> states \<and> p < length L \<and> q < length L \<and> (g1, a, r1, l1') \<in> F1 \<and> (g2, a, r2, l2') \<in> F2}"
+      using [[simproc add: finite_Collect]] by (force simp: inj_on_def intro: finite_vimageI)
+    define R where "R \<equiv> {(L, p, q, g1, g2, (a, Syn b1 b2), r1, r2, l1', l2')|L p q g1 g2 a b1 b2 r1 r2 l1' l2'.
+      L \<in> states \<and> p < length L \<and> q < length L \<and> (g1, a, b1, r1, l1') \<in> F1 \<and> (g2, a, b2, r2, l2') \<in> F2}"
 
-    have R_alt_def: "R = {t. \<exists> L p q g1 a r1 l1' g2 r2 l2'.
+    (* XXX Term for demonstrating miniscoping imperfections *)
+    term "finite
+        {t. \<exists>g1 a b1 b2 r1 l1'.
+               (g1, a, b1, r1, l1') \<in> F1 \<and>
+               (\<exists>g2 r2 l2'.
+                   (g2, a, b2, r2, l2') \<in> F2 \<and>
+                   t = (L, p, q, g1, g2, (a, Syn b1 b2), r1, r2, l1', l2'))}"
+      
+    have R_alt_def: "R = {t. \<exists> L p q g1 a b1 r1 l1' g2 b2 r2 l2'.
       L \<in> states \<and> p < length L \<and> q < length L
-      \<and> (g1, a, r1, l1') \<in> F1 \<and> (g2, a, r2, l2') \<in> F2
-      \<and> t = (L, p, q, g1, g2, a, r1, r2, l1', l2')
+      \<and> (g1, a, b1, r1, l1') \<in> F1 \<and> (g2, a, b2, r2, l2') \<in> F2
+      \<and> t = (L, p, q, g1, g2, (a, Syn b1 b2), r1, r2, l1', l2')
       }"
       unfolding R_def by auto
     have "?S \<subseteq> R" by (fastforce simp: R_alt_def F1_def F2_def states_length dest: nth_mem)
     moreover have "finite R"
       unfolding R_alt_def
       using fin1 fin2 finite_states
+      apply simp (* XXX For illustration purposes *)
       using [[simproc add: finite_Collect]]
       by (auto simp: inj_on_def intro: finite_vimageI intro!: finite_imageI)
     ultimately have "finite ?S" by (rule finite_subset)
     moreover have
       "product_trans_s
       \<subseteq> (\<lambda> (L, p, q, g1, g2, a, r1, r2, l1', l2'). (L, g1 @ g2, a, r1 @ r2, L[p := l1', q := l2'])) ` ?S"
-      unfolding product_trans_s_def apply (rule)
-       apply simp
-       apply safe[]
-      subgoal for a aa ab ac b L p q g1 g2 ad r1 r2 l1' l2'
-        apply (rule image_eqI[where x = "(L, p, q, g1, g2, ad, r1, r2, l1', l2')"])
-        by auto
-      done
+      unfolding product_trans_s_def by (simp add: image_Collect) blast
     ultimately show ?thesis by (auto intro: finite_subset)
   qed
 
@@ -574,7 +616,7 @@ lemma
 end (* End locale for product TA definition *)
 
 locale Product_TA_Defs' =
-  Product_TA_Defs N for N :: "('a, 'c, 't :: time, 's) nta"
+  Product_TA_Defs N for N :: "('a, 'b, 'c, 't :: time, 's) nta"
 begin
 
   lemma product_invariantD:
@@ -583,7 +625,7 @@ begin
   using assms unfolding product_invariant_def by (force intro: concat_guard)
 
   lemma states_step:
-    "L' \<in> states" if "N \<turnstile>\<^sub>N \<langle>L, u\<rangle> \<rightarrow> \<langle>L', u'\<rangle>" "L \<in> states"
+    "L' \<in> states" if "N \<turnstile>\<^sub>N \<langle>L, u\<rangle> \<rightarrow>\<^bsub>a\<^esub> \<langle>L', u'\<rangle>" "L \<in> states"
     using that unfolding states_def apply safe
         apply simp
        apply simp
@@ -593,7 +635,7 @@ begin
      apply rule
       apply clarsimp
     subgoal premises prems for p g a r l'
-      using prems(3,5) by force
+      using prems(3-6) by force
      apply clarsimp
      apply (auto; fail)
     apply (subst list_update_nth_split)
@@ -601,15 +643,15 @@ begin
     apply safe
      apply simp
     subgoal premises prems
-      using prems(3,6) by force
+      using prems(3-7) by force
     apply (subst list_update_nth_split)
      apply simp
     apply safe
      apply simp
     subgoal premises prems
-      using prems(3,5) by force
+      using prems(3-6) by force
     by auto
-  
+
   lemma states_steps:
     "L' \<in> states" if "N \<turnstile>\<^sub>N \<langle>L, u\<rangle> \<rightarrow>* \<langle>L', u'\<rangle>" "L \<in> states"
     using that apply (induction N \<equiv> N _ _ _ _ rule: steps_n.induct)
@@ -626,7 +668,7 @@ lemma steps_altI:
 
 (* Network + valid start state *)
 locale Product_TA =
-  Product_TA_Defs' N for N :: "('a, 'c, 't :: time, 's) nta" +
+  Product_TA_Defs' N for N :: "('a, 'b, 'c, 't :: time, 's) nta" +
   fixes L :: "'s list"
   assumes states[intro]: "L \<in> states"
 begin
@@ -635,74 +677,96 @@ begin
     len[simp]: "length L = length N"
   using states unfolding states_def by auto
 
-  lemma product_complete:
-    assumes step: "N \<turnstile>\<^sub>N \<langle>L, u\<rangle> \<rightarrow> \<langle>L', u'\<rangle>"
-    shows "product_ta \<turnstile> \<langle>L, u\<rangle> \<rightarrow> \<langle>L', u'\<rangle>"
+  lemma product_delay_complete:
+    assumes step: "N \<turnstile>\<^sub>N \<langle>L, u\<rangle> \<rightarrow>\<^bsub>Del\<^esub> \<langle>L', u'\<rangle>"
+    obtains d where "product_ta \<turnstile> \<langle>L, u\<rangle> \<rightarrow>\<^bsup>d\<^esup> \<langle>L', u'\<rangle>"
   using step proof cases
     case prems: (step_n_t d)
-    from prems(3) have *:
+    from prems have *:
       "\<forall>p\<in>{..<length N}. u \<turnstile> inv_of (N ! p) (L ! p)"
       "\<forall>p\<in>{..<length N}. u \<oplus> d \<turnstile> inv_of (N ! p) (L ! p)"
     by auto
-    from prems(1,2,4) * show ?thesis
+    from prems * show ?thesis
     by (fastforce simp add: product_ta_def inv_of_def product_invariant_def[abs_def]
-                  intro!: guard_concat
+                  intro!: guard_concat that
        )
-  next
+  qed
+
+  lemma product_int_complete:
+    assumes step: "N \<turnstile>\<^sub>N \<langle>L, u\<rangle> \<rightarrow>\<^bsub>Act b\<^esub> \<langle>L', u'\<rangle>"
+    obtains a where "product_ta \<turnstile> \<langle>L, u\<rangle> \<rightarrow>\<^bsub>(a, Act b)\<^esub> \<langle>L', u'\<rangle>"
+    using step proof cases
     case prems: (step_n_i p l g a r l')
     from prems show ?thesis
-     apply -
-     apply (rule step_a; rule step_a.intros[where g = g and r = r and a = a])
-    by (fastforce
-        simp: product_trans_def product_trans_i_def product_invariant_def product_ta_def
-              trans_of_def inv_of_def
-        intro: guard_concat
-       )+
-  next
+      apply -
+      apply (rule that)
+      apply (rule step_a.intros[where g = g and r = r])
+      by (fastforce
+          simp: product_trans_def product_trans_i_def product_invariant_def product_ta_def
+          trans_of_def inv_of_def
+          intro: guard_concat
+          )+
+  qed
+  
+  lemma product_sync_complete:
+    assumes step: "N \<turnstile>\<^sub>N \<langle>L, u\<rangle> \<rightarrow>\<^bsub>Syn b1 b2\<^esub> \<langle>L', u'\<rangle>"
+    obtains a where "product_ta \<turnstile> \<langle>L, u\<rangle> \<rightarrow>\<^bsub>(a, Syn b1 b2)\<^esub> \<langle>L', u'\<rangle>"
+    using step proof cases
     case prems: (step_n_s p l1 g1 a r1 l1' q l2 g2 r2 l2')
     from prems show ?thesis
-     apply -
-     apply (rule step_a; rule step_a.intros[where g = "g1 @ g2" and a = a and r = "r1 @ r2"])
-     subgoal premises prems
-       apply
-         (auto simp add:
-             product_trans_def product_trans_s_def product_invariant_def product_ta_def
-             trans_of_def inv_of_def
-         )
-       apply (erule allE[where x = p])
-       using \<open>p < _\<close> apply simp
-       apply (erule allE[where x = q])
-     using prems by (fastforce simp: trans_of_def)
-    by (fastforce simp: product_invariant_def product_ta_def inv_of_def intro: guard_concat)+
+      apply -
+      apply (rule that)
+      apply (rule step_a.intros[where g = "g1 @ g2" and a = "(a, Syn b1 b2)" and r = "r1 @ r2"])
+      subgoal premises prems
+        apply
+          (auto simp add:
+            product_trans_def product_trans_s_def product_invariant_def product_ta_def
+            trans_of_def inv_of_def
+            )
+        apply (erule allE[where x = p])
+        using \<open>p < _\<close> apply simp
+        apply (erule allE[where x = q])
+        using prems by (fastforce simp: trans_of_def)
+      by (fastforce simp: product_invariant_def product_ta_def inv_of_def intro: guard_concat)+
   qed
+
+  lemma product_complete:
+    assumes step: "N \<turnstile>\<^sub>N \<langle>L, u\<rangle> \<rightarrow>\<^bsub>b\<^esub> \<langle>L', u'\<rangle>"
+    shows "product_ta \<turnstile> \<langle>L, u\<rangle> \<rightarrow> \<langle>L', u'\<rangle>"
+    using step
+    by (cases b) (rule product_delay_complete product_int_complete product_sync_complete, simp, blast)+
 
   lemma product_ta_cases:
     assumes "product_ta \<turnstile> L \<longrightarrow>\<^bsup>g,a,r\<^esup> L'"
     shows "(L, g, a, r, L') \<in> product_trans_i \<or> (L, g, a, r, L') \<in> product_trans_s"
   using assms unfolding product_ta_def trans_of_def product_trans_def by auto
 
+  lemma product_delay_sound:
+    assumes step: "product_ta \<turnstile> \<langle>L, u\<rangle> \<rightarrow>\<^bsup>d\<^esup> \<langle>L', u'\<rangle>"
+    shows "N \<turnstile>\<^sub>N \<langle>L, u\<rangle> \<rightarrow>\<^bsub>Del\<^esub> \<langle>L', u'\<rangle>"
+  using assms by cases (force intro!: step_n_t product_invariantD len)
+
+  lemma product_action_sound:
+    assumes step: "product_ta \<turnstile> \<langle>L, u\<rangle> \<rightarrow>\<^bsub>(a, b)\<^esub> \<langle>L', u'\<rangle>"
+    shows "N \<turnstile>\<^sub>N \<langle>L, u\<rangle> \<rightarrow>\<^bsub>b\<^esub> \<langle>L', u'\<rangle>"
+    using assms
+    apply cases
+    apply simp
+    apply (drule product_ta_cases)
+    apply (erule disjE)
+    unfolding product_trans_i_def product_trans_s_def
+     apply (clarsimp; auto intro!: product_invariantD step_n_i; fail)
+    by (clarsimp; auto intro!: product_invariantD step_n_s)
+
   lemma product_sound:
     assumes step: "product_ta \<turnstile> \<langle>L, u\<rangle> \<rightarrow> \<langle>L', u'\<rangle>"
-    shows "N \<turnstile>\<^sub>N \<langle>L, u\<rangle> \<rightarrow> \<langle>L', u'\<rangle>"
-  using assms proof cases
-    case (step_t d)
-    then show ?thesis by (auto intro!: step_n_t product_invariantD len)
-  next
-    case (step_a a)
-    then show ?thesis
-     apply cases
-     apply simp
-     apply (drule product_ta_cases)
-     apply (erule disjE)
-     unfolding product_trans_i_def product_trans_s_def
-      apply (auto intro: product_invariantD intro!: step_n_i; fail)
-    by (auto intro: product_invariantD intro!: step_n_s)
-  qed
+    obtains a where "N \<turnstile>\<^sub>N \<langle>L, u\<rangle> \<rightarrow>\<^bsub>a\<^esub> \<langle>L', u'\<rangle>"
+    using step by cases (force dest!: product_action_sound product_delay_sound)+
 
   lemma states_product_step[intro]:
     "L' \<in> states" if "product_ta \<turnstile> \<langle>L, u\<rangle> \<rightarrow> \<langle>L', u'\<rangle>"
-    by (blast intro: product_sound states_step that)
-  
+    by (auto intro: product_sound that elim!: states_step)
+
   lemma product_steps_sound:
     "N \<turnstile>\<^sub>N \<langle>L, u\<rangle> \<rightarrow>* \<langle>L', u'\<rangle>" if "product_ta \<turnstile> \<langle>L, u\<rangle> \<rightarrow>* \<langle>L', u'\<rangle>"
     using that states proof (induction A \<equiv> product_ta _ _ _ _ rule: steps.induct)
@@ -712,27 +776,24 @@ begin
     case prems: (step l u l' u' l'' u'')
     interpret interp: Product_TA N l by standard (rule prems)
     from prems have *: "N \<turnstile>\<^sub>N \<langle>l', u'\<rangle> \<rightarrow>* \<langle>l'',u''\<rangle>" by auto
-    show ?case
-      apply (rule stepI2)
-       apply (rule *)
-      using prems by (auto intro: interp.product_sound)
+    from prems show ?case by - (erule interp.product_sound, rule stepI2, rule *)
   qed
-  
+
   lemma product_steps_complete:
     "product_ta \<turnstile> \<langle>L, u\<rangle> \<rightarrow>* \<langle>L', u'\<rangle>" if "N \<turnstile>\<^sub>N \<langle>L, u\<rangle> \<rightarrow>* \<langle>L', u'\<rangle>"
     using that states proof (induction N \<equiv> N _ _ _ _ rule: steps_n.induct)
     case (refl l Z)
     then show ?case by blast
   next
-    case prems: (step l Z l' Z' l'' Z'')
+    case prems: (step l Z l' Z' _ l'' Z'')
     interpret interp: Product_TA N l' by standard (blast intro: prems states_steps)
-    from prems show ?case by - (rule steps_altI, auto intro!: interp.product_complete)
+    from prems show ?case by - (assumption | rule steps_altI interp.product_complete)+
   qed
-  
+
   lemma product_correct:
     "product_ta \<turnstile> \<langle>L, u\<rangle> \<rightarrow>* \<langle>L', u'\<rangle> \<longleftrightarrow> N \<turnstile>\<^sub>N \<langle>L, u\<rangle> \<rightarrow>* \<langle>L', u'\<rangle>"
     by (metis product_steps_complete product_steps_sound)
-  
+
   end (* End context: network + valid start state *)
 
 end (* End of theory *)
