State_Networks.thy
@@ -1,0 +1,615 @@
+theory State_Networks
+  imports Networks Normalized_Zone_Semantics_Impl
+    "~/Formalizations/Experiments/Reordering_Quantifiers"
+begin
+
+(* XXX Move *)
+lemma finite_Collect_bounded_ex_7 [simp]:
+  assumes "finite {(a,b,c,d,e,f,g) . P a b c d e f g}"
+  shows
+    "finite {x. \<exists>a b c d e f g. P a b c d e f g \<and> Q x a b c d e f g}
+    \<longleftrightarrow> (\<forall> a b c d e f g. P a b c d e f g \<longrightarrow> finite {x. Q x a b c d e f g})"
+  using assms finite_Collect_bounded_ex[OF assms, where Q = "\<lambda> x. \<lambda> (a, b, c, d, e, f, g). Q x a b c d e f g"]
+  by clarsimp (* force, simp *)
+
+lemma finite_Collect_bounded_ex_9 [simp]:
+  assumes "finite {(a,b,c,d,e,f,g,h,i) . P a b c d e f g h i}"
+  shows
+    "finite {x. \<exists>a b c d e f g h i. P a b c d e f g h i \<and> Q x a b c d e f g h i}
+    \<longleftrightarrow> (\<forall> a b c d e f g h i. P a b c d e f g h i \<longrightarrow> finite {x. Q x a b c d e f g h i})"
+  using assms finite_Collect_bounded_ex[OF assms, where Q = "\<lambda> x. \<lambda> (a, b, c, d, e, f, g, h, i). Q x a b c d e f g h i"]
+  by clarsimp (* force, simp *)
+
+no_notation Ref.update ("_ := _" 62)
+
+section \<open>Networks of Timed Automata with Shared State\<close>
+
+subsection \<open>Syntax and Operational Semantics\<close>
+
+text \<open>
+  We extend Networks of Timed Automata with arbitrary shared (global) state.
+  Syntactically, this extension is very simple.
+  We can just use the free action label slot to annotate edges with a guard
+  and an update function on discrete states.
+  The slightly more clumsy part is adding invariants for discrete states
+  by directly specifying an invariant annotating function.
+\<close>
+
+type_synonym
+  ('a, 'c, 't, 's, 'st) snta =
+  "('a, ('st \<Rightarrow> bool) \<times> ('st \<Rightarrow> 'st), 'c, 't, 's) nta \<times> ('s \<Rightarrow> 'st \<Rightarrow> bool) list"
+
+text \<open>
+  Semantic states now consist of three things:
+  a list of process locations, the shared state, and a clock valuation.
+  The semantic extension then is also obvious: we can take the same transitions
+  as in the network without shared state, however we have to add state updates
+  and checks for guards on the shared state.
+  The updates on discrete state for synchronizing transitions are in the same order as in UPPAAL
+  (output before input).
+\<close>
+
+inductive step_sn ::
+  "('a, 'c, 't, 's, 'st) snta \<Rightarrow> 's list \<Rightarrow> 'st \<Rightarrow> ('c, ('t::time)) cval
+  \<Rightarrow> 's list \<Rightarrow> 'st \<Rightarrow> ('c, 't) cval \<Rightarrow> bool"
+  ("_ \<turnstile> \<langle>_, _, _\<rangle> \<rightarrow> \<langle>_, _, _\<rangle>" [61,61,61] 61)
+where
+  step_sn_t:
+    "(N, I) \<turnstile> \<langle>L, s, u\<rangle> \<rightarrow> \<langle>L, s, u \<oplus> d\<rangle>" if "N \<turnstile>\<^sub>N \<langle>L, u\<rangle> \<rightarrow>\<^bsub>Del\<^esub> \<langle>L, u \<oplus> d\<rangle>" "length N = length I" |
+  step_sn_i:
+    "(N, I) \<turnstile> \<langle>L, s, u\<rangle> \<rightarrow> \<langle>L', s', u'\<rangle>"
+    if "N \<turnstile>\<^sub>N \<langle>L, u\<rangle> \<rightarrow>\<^bsub>Act (c, m)\<^esub> \<langle>L', u'\<rangle>" "c s" "\<forall> p < length I. (I ! p) (L' ! p) s'" "s' = m s"
+       "length N = length I" |
+  step_sn_s:
+    "(N, I) \<turnstile> \<langle>L, s, u\<rangle> \<rightarrow> \<langle>L', s', u'\<rangle>"
+    if "N \<turnstile>\<^sub>N \<langle>L, u\<rangle> \<rightarrow>\<^bsub>Syn (ci, mi) (co, mo)\<^esub> \<langle>L', u'\<rangle>"
+       "ci s" "co s" "\<forall> p < length I. (I ! p) (L' ! p) s'"
+       "s' = mi (mo s)" "length N = length I"
+
+inductive_cases[elim!]: "N \<turnstile> \<langle>L, s, u\<rangle> \<rightarrow> \<langle>L', s', u'\<rangle>"
+
+inductive steps_sn ::
+  "('a, 'c, 't, 's, 'st) snta \<Rightarrow> 's list \<Rightarrow> 'st \<Rightarrow> ('c, ('t::time)) cval
+  \<Rightarrow> 's list \<Rightarrow> 'st \<Rightarrow> ('c, 't) cval \<Rightarrow> bool"
+("_ \<turnstile> \<langle>_, _, _\<rangle> \<rightarrow>* \<langle>_, _, _\<rangle>" [61, 61, 61,61,61] 61)
+where
+  refl: "N \<turnstile> \<langle>L, s, u\<rangle> \<rightarrow>* \<langle>L, s, u\<rangle>" |
+  step: "N \<turnstile> \<langle>L, s, u\<rangle> \<rightarrow>* \<langle>L', s', u'\<rangle> \<Longrightarrow> N \<turnstile> \<langle>L', s', u'\<rangle> \<rightarrow> \<langle>L'', s'', u''\<rangle>
+        \<Longrightarrow> N \<turnstile> \<langle>L, s, u\<rangle> \<rightarrow>* \<langle>L'', s'', u''\<rangle>"
+
+declare steps_sn.intros[intro]
+
+lemma stepI2:
+  "N \<turnstile> \<langle>l, s, u\<rangle> \<rightarrow>* \<langle>l'', s'', u''\<rangle>" if
+  "N \<turnstile> \<langle>l', s', u'\<rangle> \<rightarrow>* \<langle>l'', s'', u''\<rangle>" "N \<turnstile> \<langle>l, s, u\<rangle> \<rightarrow> \<langle>l', s', u'\<rangle>"
+  using that
+  apply induction
+   apply rule
+    apply (rule refl)
+   apply assumption
+  apply simp
+  by (rule; assumption)
+
+subsection \<open>Product Automaton\<close>
+
+(*
+abbreviation state_set :: "('a, 'c, 'time, 's) transition set \<Rightarrow> 's set" where
+  "state_set T \<equiv> fst ` T \<union> (snd o snd o snd o snd) ` T"
+*)
+
+locale Prod_TA_Defs =
+  fixes A :: "('a, 'c, 't, 's, 'st) snta"
+begin
+
+  interpretation Product_TA_Defs "fst A" .
+
+term product_ta
+
+  abbreviation "N \<equiv> fst A"
+  abbreviation "P \<equiv> snd A"
+  abbreviation "T' \<equiv> trans_of product_ta"
+  abbreviation "I' \<equiv> inv_of product_ta"
+
+  definition "p \<equiv> length N"
+
+  (* definition "states = {L. length L = length T \<and> (\<forall> p \<in> {..<length T}. L!p \<in> state_set (T!p))}" *)
+
+  definition
+    "prod_trans_i =
+      {((L, s), g, a, r, (L', m s)) | L s g c a r m L'.
+       (\<forall> q < p. (P ! q) (L ! q) s) \<and> (\<forall> q < p. (P ! q) (L' ! q) (m s))
+       \<and> (L, g, (a, Act (c, m)), r, L') \<in> T' \<and> c s}"
+
+  definition
+    "prod_trans_s =
+      {((L, s), g, a, r, (L', s')) | L s g ci co a r mi mo L' s'.
+        ci s \<and> co s
+        \<and> (\<forall> q < p. (P ! q) (L ! q) s) \<and> (\<forall> q < p. (P ! q) (L' ! q) s')
+        \<and> (L, g, (a, Syn (ci, mi) (co, mo)), r, L') \<in> T'
+        \<and> s' = mi (mo s)
+      }"
+
+  definition
+    "prod_trans \<equiv> prod_trans_i \<union> prod_trans_s"
+
+  definition
+    "prod_invariant \<equiv> product_invariant o fst"
+
+  definition prod_ta :: "('a, 'c, 't, 's list \<times> 'st) ta" where
+    "prod_ta \<equiv> (prod_trans, prod_invariant)"
+
+  lemma prod_ta_cases:
+    assumes "prod_ta \<turnstile> L \<longrightarrow>\<^bsup>g,a,r\<^esup> L'"
+    shows "(L, g, a, r, L') \<in> prod_trans_i \<or> (L, g, a, r, L') \<in> prod_trans_s"
+    using assms unfolding prod_ta_def trans_of_def prod_trans_def by auto
+
+  lemma inv_of_simp:
+    "inv_of prod_ta (L, s) = I' L"
+    unfolding inv_of_def prod_ta_def prod_invariant_def product_ta_def by simp
+
+  lemma collect_clki_prod_invariant:
+    "collect_clki prod_invariant = collect_clki product_invariant"
+    unfolding prod_invariant_def collect_clki_def by simp
+
+  (*
+  lemma states_length:
+    assumes "L \<in> states"
+    shows "length L = length N"
+    using assms unfolding states_def by auto
+    *)
+
+  lemma collect_clkt_prod_trans_subs:
+    "collect_clkt prod_trans \<subseteq> collect_clkt T'"
+    unfolding collect_clkt_def prod_trans_def prod_trans_i_def prod_trans_s_def by fastforce
+
+  lemma collect_clkvt_prod_trans_subs:
+    "collect_clkvt prod_trans \<subseteq> collect_clkvt T'"
+    unfolding collect_clkvt_def prod_trans_def prod_trans_i_def prod_trans_s_def by fastforce
+
+  (* XXX No conditional split *)
+  (*
+  lemma statesI_aux:
+    fixes L
+    assumes L: "L \<in> states"
+    assumes
+      "p < length T"
+      "(l, g, a, r, l') \<in> T ! p"
+    shows "(L[p := l]) \<in> states"
+    unfolding states_def apply clarsimp
+    apply rule
+    using L apply (simp add: states_def)
+    apply rule
+    apply (subst list_update_nth_split)
+    using assms apply (auto simp: states_def)
+    by blast
+*)
+(*
+  lemma product_trans_s_alt_def:
+    "product_trans_s =
+      {(L, g, a, r, L') | L g a r L'. \<exists> p q g1 g2 r1 r2 l1' l2'.
+      L \<in> states \<and> p < length L \<and> q < length L \<and> p \<noteq> q \<and>
+      g = g1 @ g2 \<and> r = r1 @ r2 \<and> L' = L[p:=l1', q:=l2']
+        \<and> (L!p, g1, In a, r1, l1') \<in> T!p \<and> (L!q, g2, Out a, r2, l2') \<in> T!q
+      }"
+    unfolding product_trans_s_def by (safe; metis)
+*)
+  (*
+  context
+    assumes states_not_empty: "states \<noteq> {}"
+    assumes trans_complete:
+      "\<forall> p < length T. \<forall> t1 \<in> T ! p. case t1 of (l1, g1, In a, r1, l1')
+      \<Rightarrow> \<exists> q < length T. p \<noteq> q \<and> (\<exists> l2 g2 r2 l2'. (l2, g2, Out a, r2, l2') \<in> T ! q) |
+      (l1, g1, Out a, r1, l1')
+      \<Rightarrow> \<exists> q < length T. p \<noteq> q \<and> (\<exists> l2 g2 r2 l2'. (l2, g2, In a, r2, l2') \<in> T ! q) | _ \<Rightarrow> True"
+  begin
+
+  lemma collect_clkt_product_trans_sups:
+    "collect_clkt product_trans \<supseteq> \<Union> (collect_clkt ` set T)"
+  proof
+    fix x assume "x \<in> \<Union> (collect_clkt ` set T)"
+    then obtain trans l1 g1 a' r1 l1' where x:
+      "trans \<in> set T" "(l1, g1, a', r1, l1') \<in> trans" "x \<in> collect_clock_pairs g1"
+      unfolding collect_clkt_def by force
+    then obtain p where p:
+        "p < length T" "T ! p = trans"
+      by (auto dest!: aux)
+    from states_not_empty obtain L where L: "L \<in> states" by auto
+    have "length T = length L" by (auto simp: states_length[OF \<open>L \<in> states\<close>])
+    show "x \<in> collect_clkt product_trans"
+    proof (cases a')
+      case a': (In a)
+      with x p trans_complete obtain q l2 g2 r2 l2' where trans2:
+        "q < length T" "(l2, g2, Out a, r2, l2') \<in> T ! q" "p \<noteq> q"
+        by atomize_elim fastforce
+      have "L[p := l1, q := l2] \<in> states" (is "?L \<in> _")
+        using L p(1) x(1,2) trans2 unfolding p(2)[symmetric] by (auto intro!: statesI_aux)
+      moreover have "?L ! p = l1" "?L ! q = l2"
+        using \<open>p \<noteq> q\<close> \<open>p < length T\<close> \<open>q < length T\<close> \<open>L \<in> states\<close> by (auto dest: states_length)
+      moreover note t = calculation
+      have "(?L, g1 @ g2, a, r1 @ r2, ?L[p := l1', q := l2']) \<in> product_trans_s"
+        unfolding product_trans_s_alt_def
+        apply clarsimp
+        using t p(1) x(1,2) trans2 unfolding p(2)[symmetric] a' \<open>length T = length L\<close>
+        by metis
+      moreover have "x \<in> collect_clock_pairs (g1 @ g2)"
+        using x(3) by (auto simp: collect_clock_pairs_def)
+      ultimately show ?thesis unfolding collect_clkt_def product_trans_def by force
+    next
+      case a': (Out a)
+      with x p trans_complete obtain q l2 g2 r2 l2' where trans2:
+        "q < length T" "(l2, g2, In a, r2, l2') \<in> T ! q" "p \<noteq> q"
+        by atomize_elim fastforce
+      have "L[q := l2, p := l1] \<in> states" (is "?L \<in> _")
+        using L p(1) x(1,2) trans2 unfolding p(2)[symmetric] by (auto intro!: statesI_aux)
+      moreover have "?L ! p = l1" "?L ! q = l2"
+        using \<open>p \<noteq> q\<close> \<open>p < length T\<close> \<open>q < length T\<close> \<open>L \<in> states\<close> by (auto dest: states_length)
+      moreover note t = calculation
+      have "(?L, g2 @ g1, a, r2 @ r1, ?L[q := l2', p := l1']) \<in> product_trans_s"
+        unfolding product_trans_s_alt_def
+        apply clarsimp
+        using t p(1) x(1,2) trans2 unfolding p(2)[symmetric] a' \<open>length T = length L\<close>
+        by metis
+      moreover have "x \<in> collect_clock_pairs (g2 @ g1)"
+        using x(3) by (auto simp: collect_clock_pairs_def)
+      ultimately show ?thesis unfolding collect_clkt_def product_trans_def by force
+    next
+      case a': (Sil a)
+      have "L[p := l1] \<in> states" (is "?L \<in> _")
+        using L p(1) x(1,2) unfolding p(2)[symmetric] by (auto intro!: statesI_aux)
+      moreover have "?L ! p = l1"
+        using \<open>p < length T\<close> \<open>L \<in> states\<close> by (auto dest: states_length)
+      ultimately have "(?L, g1, a, r1, ?L[p := l1']) \<in> product_trans_i"
+        using x p unfolding product_trans_i_def a' by (force simp: states_length[OF \<open>L \<in> states\<close>])
+      with x(3) show ?thesis unfolding collect_clkt_def product_trans_def by force
+    qed
+  qed
+
+  lemma collect_clkvt_product_trans_sups:
+    "collect_clkvt product_trans \<supseteq> \<Union> (collect_clkvt ` set T)"
+  proof
+    fix x assume "x \<in> \<Union> (collect_clkvt ` set T)"
+    then obtain trans l1 g1 a' r1 l1' where x:
+      "trans \<in> set T" "(l1, g1, a', r1, l1') \<in> trans" "x \<in> set r1"
+      unfolding collect_clkvt_def by force
+    then obtain p where p:
+        "p < length T" "T ! p = trans"
+      by (auto dest!: aux)
+    from states_not_empty obtain L where L: "L \<in> states" by auto
+    show "x \<in> collect_clkvt product_trans"
+    proof (cases a')
+      case a': (In a)
+      with x p trans_complete obtain q l2 g2 r2 l2' where trans2:
+        "q < length T" "(l2, g2, Out a, r2, l2') \<in> T ! q" "p \<noteq> q"
+        by atomize_elim fastforce
+      moreover have "L[p := l1, q := l2] \<in> states" (is "?L \<in> _")
+        using L p(1) x(1,2) trans2 unfolding p(2)[symmetric] by (auto intro!: statesI_aux)
+      moreover have "?L ! p = l1" "?L ! q = l2"
+        using \<open>p \<noteq> q\<close> \<open>p < length T\<close> \<open>q < length T\<close> \<open>L \<in> states\<close> by (auto dest: states_length)
+      ultimately have "(?L, g1 @ g2, a, r1 @ r2, ?L[p := l1', q := l2']) \<in> product_trans_s"
+        using p(1) x trans2 unfolding p(2)[symmetric] a' product_trans_s_def
+        by (fastforce simp: states_length[OF \<open>L \<in> states\<close>])
+      with x(3) show ?thesis unfolding collect_clkvt_def product_trans_def by force
+    next
+      case a': (Out a)
+      with x p trans_complete obtain q l2 g2 r2 l2' where trans2:
+        "q < length T" "(l2, g2, In a, r2, l2') \<in> T ! q" "p \<noteq> q"
+        by atomize_elim fastforce
+      moreover have "L[q := l2, p := l1] \<in> states" (is "?L \<in> _")
+        using L p(1) x(1,2) trans2 unfolding p(2)[symmetric] by (auto intro!: statesI_aux)
+      moreover have "?L ! p = l1" "?L ! q = l2"
+        using \<open>p \<noteq> q\<close> \<open>p < length T\<close> \<open>q < length T\<close> \<open>L \<in> states\<close> by (auto dest: states_length)
+      ultimately have "(?L, g2 @ g1, a, r2 @ r1, ?L[q := l2', p := l1']) \<in> product_trans_s"
+        using p(1) x trans2 unfolding p(2)[symmetric] a' product_trans_s_def
+        by (fastforce simp: states_length[OF \<open>L \<in> states\<close>])
+      with x(3) show ?thesis unfolding collect_clkvt_def product_trans_def by force
+    next
+      case a': (Sil a)
+      have "L[p := l1] \<in> states" (is "?L \<in> _")
+        using L p(1) x(1,2) unfolding p(2)[symmetric] by (auto intro!: statesI_aux)
+      moreover have "?L ! p = l1"
+        using \<open>p < length T\<close> \<open>L \<in> states\<close> by (auto dest: states_length)
+      ultimately have "(?L, g1, a, r1, ?L[p := l1']) \<in> product_trans_i"
+        using x p unfolding product_trans_i_def a' by (force simp: states_length[OF \<open>L \<in> states\<close>])
+      with x(3) show ?thesis unfolding collect_clkvt_def product_trans_def by force
+    qed
+  qed
+
+  lemma collect_clkt_product_trans:
+    "collect_clkt product_trans = \<Union> (collect_clkt ` set T)"
+    using collect_clkt_product_trans_sups collect_clkt_product_trans_subs by simp
+
+  lemma collect_clkvt_product_trans:
+    "collect_clkvt product_trans = \<Union> (collect_clkvt ` set T)"
+  using collect_clkvt_product_trans_sups collect_clkvt_product_trans_subs by simp
+
+  end (* End of context for syntactic 1-to-1 correspondence for transitions *)
+*)
+
+term N term P
+
+lemma T_simp:
+  "T ! q = trans_of (N ! q)" if "q < length N"
+  using that by simp
+
+lemma prod_state_set_subs:
+  assumes "l \<in> state_set T'" "q < p"
+  shows "l ! q \<in> state_set (trans_of (N ! q))"
+  using assms
+  apply (simp only: T_simp[symmetric] p_def)
+  by (rule product_state_set_subs; simp add: product_ta_def trans_of_def)
+
+context
+  assumes finite_state:
+    "\<forall> q < p. \<forall> l \<in> state_set (trans_of (N ! q)). finite {s. (P ! q) l s}"
+      and finite_trans: "\<forall> A \<in> set N. finite (trans_of A)"
+begin
+
+lemma finite_state':
+  "\<forall> q < p. \<forall> l \<in> state_set T'. finite {s. (P ! q) (l ! q) s}"
+  using finite_state prod_state_set_subs by simp
+
+lemma finite_state'':
+  "finite {s. \<forall> q < p. (P ! q) (l ! q) s}" if \<open>p > 0\<close> \<open>l \<in> state_set T'\<close>
+proof -
+  from \<open>p > 0\<close> obtain q where "q < p" by auto
+  with finite_state' \<open>l \<in> _\<close> have "finite {s. (P ! q) (l ! q) s}" by auto
+  then show ?thesis by (rule rev_finite_subset) (auto intro: \<open>q < p\<close>)
+qed
+
+lemma prod_trans_i_alt_def:
+  "prod_trans_i =
+    {((L, s), g, a, r, (L', m s)) | L s g c a r m L'.
+     (L, g, (a, Act (c, m)), r, L') \<in> T' \<and>
+     (\<forall> q < p. (P ! q) (L ! q) s) \<and> (\<forall> q < p. (P ! q) (L' ! q) (m s))
+     \<and> c s}"
+  unfolding prod_trans_i_def by (safe; metis)
+
+lemma finite_prod_trans:
+  "finite prod_trans" if "p > 0"
+  unfolding prod_trans_def prod_trans_i_alt_def prod_trans_s_def
+  apply safe
+  subgoal
+    apply (tactic \<open>defer_ex_tac @{context} 1\<close>, simp only: conj_assoc)
+    using [[simproc add: ex_reorder4]]
+    apply simp
+    apply (subst finite_Collect_bounded_ex_7)
+    subgoal
+      using [[simproc add: finite_Collect]] finite_trans_of_product[OF finite_trans]
+      by (auto intro!: finite_imageI finite_vimageI simp: inj_on_def)
+    apply safe
+    (* When unfolding regular_def
+    apply (tactic \<open>defer_ex_tac @{context} 1\<close>) (* XXX *)
+    *)
+    apply (subst finite_Collect_bounded_ex)
+    by (auto intro: finite_state'' \<open>p > 0\<close>)
+  subgoal
+    apply (tactic \<open>defer_ex_tac @{context} 1\<close>, simp only: conj_assoc)
+    apply (tactic \<open>rearrange_ex_fixed_5 @{context} 1\<close>)
+    apply (use [[simproc add: ex_reorder4]] in simp)
+    apply (subst finite_Collect_bounded_ex_9)
+    subgoal
+      using [[simproc add: finite_Collect]] finite_trans_of_product[OF finite_trans]
+      by (auto intro!: finite_imageI finite_vimageI simp: inj_on_def)
+    apply (tactic \<open>defer_ex_tac @{context} 1\<close>, simp only: conj_assoc)
+    apply (tactic \<open>defer_ex_tac @{context} 1\<close>, simp only: conj_assoc)
+    apply safe
+    apply (subst finite_Collect_bounded_ex)
+    by (auto intro: finite_state'' \<open>p > 0\<close>)
+  done
+
+thm finite_product_trans_i[OF finite_trans] finite_product_trans_s[OF finite_trans]
+
+thm finite_trans_of_product[OF finite_trans]
+thm finite_states
+
+end (* End of context for finiteness of automaton *)
+
+end (* End locale for product TA definition *)
+
+locale Prod_TA_Defs' =
+  Prod_TA_Defs A for A :: "('a, 'c, 't :: time, 's, 'st) snta"
+begin
+
+  interpretation Product_TA_Defs' "fst A".
+
+  thm Networks.Product_TA_Defs'.product_invariantD product_invariantD
+
+  term "step_sn A" term states
+
+  lemma states_step:
+    "L' \<in> states" if "A \<turnstile> \<langle>L, s, u\<rangle> \<rightarrow> \<langle>L', s', u'\<rangle>" "L \<in> states"
+    using that states_step by cases auto
+
+  lemma states_steps:
+    "L' \<in> states" if "A \<turnstile> \<langle>L, s, u\<rangle> \<rightarrow>* \<langle>L', s', u'\<rangle>" "L \<in> states"
+    using that apply (induction A \<equiv> A _ _ _ _ _ _ rule: steps_sn.induct)
+     apply assumption
+    apply simp
+    by (rule states_step)
+
+  lemma inv_step:
+    "\<forall>p<length P. (P ! p) (L' ! p) s'" if
+    "A \<turnstile> \<langle>L, s, u\<rangle> \<rightarrow> \<langle>L', s', u'\<rangle>" "\<forall>p<length P. (P ! p) (L ! p) s"
+    using that by (cases) auto
+
+  lemma inv_steps:
+    "\<forall>p<length P. (P ! p) (L' ! p) s'" if
+    "A \<turnstile> \<langle>L, s, u\<rangle> \<rightarrow>* \<langle>L', s', u'\<rangle>" "\<forall>p<length P. (P ! p) (L ! p) s"
+    using that apply (induction A \<equiv> A _ _ _ _ _ _ rule: steps_sn.induct) by (auto intro: inv_step)
+
+end
+
+thm steps_altI
+
+(* Network + valid start state *)
+locale Prod_TA =
+  Prod_TA_Defs A for A :: "('a, 'c, 't :: time, 's, 'st) snta" +
+  fixes L :: "'s list"
+  assumes states[intro]: "L \<in> Product_TA_Defs.states N"
+  fixes s :: 'st
+  assumes Len: "length N = length P"
+      and inv: "\<forall>p<length P. (P ! p) (L ! p) s"
+begin
+
+  interpretation Product_TA N L by standard rule
+
+  term product_ta
+
+  lemma product_inv_prod[intro]:
+    "u \<turnstile> inv_of prod_ta (l, s')" if "u \<turnstile> inv_of product_ta l"
+    using that unfolding product_ta_def prod_ta_def prod_invariant_def inv_of_def by auto
+
+  lemma A_simp[simp]:
+    "N' = N" "P' = P" if "A = (N', P')"
+    using that by auto
+
+  lemma prod_complete:
+    assumes step: "A \<turnstile> \<langle>L, s, u\<rangle> \<rightarrow> \<langle>L', s', u'\<rangle>"
+    shows "prod_ta \<turnstile> \<langle>(L, s), u\<rangle> \<rightarrow> \<langle>(L', s'), u'\<rangle>"
+  using step proof cases
+    case (step_sn_t N d P)
+    then show ?thesis
+      apply -
+      apply (frule A_simp)
+      apply (drule A_simp(2))
+      by (force elim!: product_delay_complete)
+  next
+    case prems: (step_sn_i N c m I)
+    note [simp] = A_simp[OF prems(1)]
+    from prems(6) have [simp]: "length P = p" by (simp add: p_def)
+    from prems(2-) obtain a where "product_ta \<turnstile> \<langle>L, u\<rangle> \<rightarrow>\<^bsub>(a, Act (c, m))\<^esub> \<langle>L', u'\<rangle>"
+      by (auto elim!: product_int_complete)
+    with prems(3-5) inv obtain g r where step:
+        "((L, s), g, a, r, (L', s')) \<in> prod_trans_i"
+        "u \<turnstile> g" "u' = [r\<rightarrow>0]u" "u' \<turnstile> inv_of product_ta L'"
+      unfolding prod_trans_i_def by - (erule step_a.cases; auto)
+    then have "((L, s), g, a, r, (L', s')) \<in> trans_of prod_ta"
+      by (simp add: prod_trans_def trans_of_def prod_ta_def)
+    then show ?thesis
+      apply -
+      apply (rule step_a)
+      apply rule
+      using step(2-) by force+
+  next
+    case prems: (step_sn_s N ci mi co mo I)
+    note [simp] = A_simp[OF prems(1)]
+    from prems(7) have [simp]: "length P = p" by (simp add: p_def)
+    from prems(2-) obtain a where "product_ta \<turnstile> \<langle>L, u\<rangle> \<rightarrow>\<^bsub>(a, Syn (ci, mi) (co, mo))\<^esub> \<langle>L', u'\<rangle>"
+      by (auto elim!: product_sync_complete)
+    with prems(3-6) inv obtain g r where step:
+        "((L, s), g, a, r, (L', s')) \<in> prod_trans_s"
+        "u \<turnstile> g" "u' = [r\<rightarrow>0]u" "u' \<turnstile> inv_of product_ta L'"
+      unfolding prod_trans_s_def by - (erule step_a.cases; auto; blast)
+        (* XXX Simproc for instantiations from equality? *)
+    then have "((L, s), g, a, r, (L', s')) \<in> trans_of prod_ta"
+      by (simp add: prod_trans_def trans_of_def prod_ta_def)
+    then show ?thesis
+      apply -
+      apply (rule step_a)
+      apply rule
+      using step(2-) by force+
+  qed
+
+  lemma A_unfold:
+    "A = (N, P)"
+    by simp
+
+  thm states_step
+
+  lemma prod_sound:
+    assumes step: "prod_ta \<turnstile> \<langle>(L, s), u\<rangle> \<rightarrow> \<langle>(L', s'), u'\<rangle>"
+    shows "A \<turnstile> \<langle>L, s, u\<rangle> \<rightarrow> \<langle>L', s', u'\<rangle>"
+    using assms proof cases
+    case (step_t d)
+    then show ?thesis
+    proof cases
+      case prems: 1
+      then have "product_ta \<turnstile> \<langle>L, u\<rangle> \<rightarrow>\<^bsup>d\<^esup> \<langle>L', u'\<rangle>" unfolding inv_of_simp by fast
+      from product_delay_sound[OF this] prems show ?thesis
+        apply simp
+        apply (subst A_unfold)
+        apply (rule step_sn_t)
+        by (simp add: Len)+
+    qed
+  next
+    case (step_a a)
+    from Len have [simp]: "length P = p" by (simp add: p_def)
+    from step_a show ?thesis
+    proof cases
+      case prems: (1 g r)
+      from this(1) show ?thesis
+        apply -
+      proof (drule prod_ta_cases, erule disjE, goal_cases)
+        case 1
+        then obtain c m where *:
+          "s' = m s" "\<forall>q<p. (P ! q) (L ! q) s"
+          "\<forall>q<p. (P ! q) (L' ! q) (m s)" "product_ta \<turnstile> L \<longrightarrow>\<^bsup>g,(a, Act (c, m)),r\<^esup> L'" "c s"
+          unfolding prod_trans_i_def by force
+        with prems have "product_ta \<turnstile> \<langle>L, u\<rangle> \<rightarrow>\<^bsub>(a, Act (c, m))\<^esub> \<langle>L', u'\<rangle>"
+          unfolding inv_of_simp by - rule
+        from product_action_sound[OF this] prems * show ?thesis
+          apply (subst A_unfold)
+          apply (rule step_sn_i)
+          by (simp add: Len)+
+      next
+        case 2
+        then obtain ci co mi mo where *:
+          "s' = mi (mo s)" "\<forall>q<p. (P ! q) (L ! q) s"
+          "\<forall>q<p. (P ! q) (L' ! q) s'" "product_ta \<turnstile> L \<longrightarrow>\<^bsup>g,(a, Syn (ci, mi) (co, mo)),r\<^esup> L'"
+          "ci s" "co s"
+          unfolding prod_trans_s_def by auto
+        with prems have "product_ta \<turnstile> \<langle>L, u\<rangle> \<rightarrow>\<^bsub>(a, Syn (ci, mi) (co, mo))\<^esub> \<langle>L', u'\<rangle>"
+          unfolding inv_of_simp by - rule
+        from product_action_sound[OF this] prems * show ?thesis
+          apply (subst A_unfold)
+          apply (rule step_sn_s)
+          by (simp add: Len)+
+      qed
+    qed
+  qed
+
+  lemma states_prod_step[intro]:
+    "L' \<in> states" if "prod_ta \<turnstile> \<langle>(L, s), u\<rangle> \<rightarrow> \<langle>(L', s'), u'\<rangle>"
+    sorry
+
+  lemma inv_prod_step[intro]:
+    "\<forall>p<length P. (P ! p) (L' ! p) s'" if "prod_ta \<turnstile> \<langle>(L, s), u\<rangle> \<rightarrow> \<langle>(L', s'), u'\<rangle>"
+    sorry
+
+  lemma prod_steps_sound:
+    assumes step: "prod_ta \<turnstile> \<langle>(L, s), u\<rangle> \<rightarrow>* \<langle>(L', s'), u'\<rangle>"
+    shows "A \<turnstile> \<langle>L, s, u\<rangle> \<rightarrow>* \<langle>L', s', u'\<rangle>"
+    using step states inv
+  proof (induction A \<equiv> prod_ta l \<equiv> "(L, s)" _ l' \<equiv> "(L', s')" _ arbitrary: L s rule: steps.induct)
+    case (refl u)
+    then show ?case by blast
+  next
+    case prems: (step u l' u' u'' L s)
+    obtain L'' s'' where "l' = (L'', s'')" by force
+    interpret interp: Prod_TA A L s by (standard; rule prems Len)
+    from prems(3)[OF \<open>l' = _\<close>] prems(1,2,4-) have *: "A \<turnstile> \<langle>L'', s'', u'\<rangle> \<rightarrow>* \<langle>L', s', u''\<rangle>"
+      unfolding \<open>l' = _\<close> using  interp.inv_prod_step by auto
+    show ?case
+      apply (rule stepI2)
+      using * prems by (auto simp: \<open>l' = _\<close> intro: interp.prod_sound)
+  qed
+
+  lemma prod_steps_complete:
+    "prod_ta \<turnstile> \<langle>(L, s), u\<rangle> \<rightarrow>* \<langle>(L', s'), u'\<rangle>" if "A \<turnstile> \<langle>L, s, u\<rangle> \<rightarrow>* \<langle>L', s', u'\<rangle>"
+    using that states inv proof (induction A \<equiv> A L _ _ _ _ _ rule: steps_sn.induct)
+    case (refl L s u)
+    then show ?case by blast
+  next
+    case prems: (step L s u L' s' u' L'' s'' u'')
+    interpret interp: Prod_TA A L' s' apply standard
+      using prems by - (assumption | rule Prod_TA_Defs'.states_steps Len Prod_TA_Defs'.inv_steps)+
+    from prems show ?case by - (rule steps_altI, auto intro!: interp.prod_complete)
+  qed
+
+  lemma prod_correct:
+    "prod_ta \<turnstile> \<langle>(L, s), u\<rangle> \<rightarrow>* \<langle>(L', s'), u'\<rangle> \<longleftrightarrow> A \<turnstile> \<langle>L, s, u\<rangle> \<rightarrow>* \<langle>L', s', u'\<rangle>"
+    by (metis prod_steps_complete prod_steps_sound)
+
+  end (* End context: network + valid start state *)
+
+end (* End of theory *)
